fixes coop case study

theories/case_studies/cooperative_concurrency.v
@@ -118,125 +118,116 @@ Section typing.
   Definition coop_pre (θ : sem_row Σ) : sem_row Σ := 
     (("async", async_sig θ) · ("await", await_sig) · ⟨⟩)%R.
 
+
   Local Instance await_sig_ne :
     NonExpansive (λ (α : sem_ty Σ), Promise (! α)).
   Proof.
-    rewrite /Promise /Status. intros ?????.
-    apply non_dep_fun_dist. by repeat f_equiv.
+    rewrite /Promise /Status. 
+    intros ????. by repeat f_equiv.
   Qed.
 
   Local Instance async_sig_ne θ :
-    NonExpansive
-      (λ (α : sem_ty Σ), 𝟙 -{ θ }-∘ ! α).
+    NonExpansive (λ (α : sem_ty Σ), 𝟙 -{ θ }-∘ ! α).
   Proof.
-    intros ?????. apply non_dep_fun_dist.
-    do 2 f_equiv; try done. 
+    intros ????. by repeat f_equiv.
   Qed.
 
   Local Instance async_sig_2_ne : NonExpansive async_sig.
   Proof.
-    intros ?????. rewrite /async_sig. apply non_dep_fun_dist.
-    f_equiv. rewrite /tele_app. simpl. intros ?. destruct x0. simpl;
-    f_equiv.
+    rewrite /async_sig.
+    intros ?????. apply non_dep_fun_dist.
+ f_equiv. rewrite /tele_app. intros []; simpl; apply non_dep_fun_dist;
+    repeat f_equiv; intros ?; by repeat f_equiv.
   Qed.
 
   Local Instance contractive_coop_pre : Contractive coop_pre.
   Proof. 
-    intros ????. rewrite /coop_pre. f_equiv. f_equiv. f_equiv. 
+    intros ????. rewrite /coop_pre. do 3 f_equiv. 
     destruct n; first apply dist_later_0.
     apply dist_later_S. rewrite - dist_later_S in H.
     by f_equiv.
   Qed.
 
-  Definition coop : sem_row Σ := (μR: θ, coop_pre θ)%R.
+  Definition coop : sem_row Σ := (μᵣ θ, coop_pre θ)%R.
 
   Local Instance await_res_sig_ne :
-    NonExpansive
-      (λ (α : sem_ty Σ), '! α).
-  Proof.
-    intros ????. by repeat f_equiv.
-  Qed.
+    NonExpansive (λ (α : sem_ty Σ), ! α).
+  Proof. intros ????. by repeat f_equiv. Qed.
 
-  Local Instance coop_os_row : Once coop.
-  Proof.
-    rewrite /coop. apply row_rec_once. iIntros (θ).
-    rewrite /coop_pre. apply row_cons_once.
-    { rewrite /async_sig. apply sig_eff_os_once; apply _. }
-    apply row_cons_once; last apply row_nil_once.
-    apply sig_eff_os_once; apply _.
-  Qed.
+  Local Instance coop_os_row : OnceR coop.
+  Proof. apply _. Qed.
 
-  Definition iter_ty τ := (∀R: θ, (τ -{ ¡ θ }-> 𝟙) → List τ -{ ¡ θ }-∘ 𝟙)%T.
+  Definition iter_ty τ := (∀ᵣ θ, (τ -{ ¡ θ }-> 𝟙) → List τ -{ ¡ θ }-∘ 𝟙)%T.
   
   Definition next_ty := (𝟙 → 𝟙)%T.
 
   Definition add_ty := ((𝟙 ⊸ 𝟙) → 𝟙)%T.
 
-  Definition resume_task_ty := (∀T: α, '! α → ('! α ⊸ 𝟙) → 𝟙)%T.
+  Definition resume_task_ty := (∀ₜ α, ! α → (! α ⊸ 𝟙) → 𝟙)%T.
   
-  Definition runner_ty := (∀T: α, (𝟙 -{ coop }-∘ '! α) → '! α)%T.
+  Definition runner_ty := (∀ₜ α, (𝟙 -{ coop }-∘ ! α) → ! α)%T.
 
   Lemma impossible_typed τ :
-    ⊢ ⊨ impossible : ⊥ : τ.
+    ⊢ ⊨ impossible : ⟨⟩ : τ.
   Proof.
     iIntros. rewrite /impossible.
     iApply sem_typed_app_os; [|iApply sem_typed_unit].
     rewrite - {1} (app_nil_r []).
     iApply sem_typed_sub_u2aarr.
-    iApply sem_typed_ufun; solve_sidecond. simpl.
+    smart_apply sem_typed_ufun. simpl.
     iApply sem_typed_app_os; [|iApply sem_typed_unit].
     iApply sem_typed_sub_u2aarr.
     iApply sem_typed_var.
   Qed.
 
   Lemma async_typed :
-    ⊢ ⊨ᵥ async : (∀T: α, (𝟙 -{ coop }-∘ '! α) -{ coop }-> Promise ('! α)).
+    ⊢ ⊨ᵥ async : (∀ₜ α, (𝟙 -{ coop }-∘ ! α) -{ coop }-> Promise (! α)).
   Proof.
     rewrite /async. iIntros.
     iApply sem_typed_Tclosure. iIntros (α).
-    iApply sem_typed_closure; solve_sidecond. simpl. rewrite /coop.
+    smart_apply sem_typed_closure. simpl. rewrite /coop.
     iApply sem_typed_sub_row; first iApply row_le_rec_fold.
     rewrite /coop_pre -/coop.
     iApply (sem_typed_perform_os (TT:=[tele _]) [tele_arg (α : sem_ty Σ)] _ "async"
-                                 (tele_app (λ α, 𝟙 -{ coop }-∘ '! α)) (tele_app (λ α, Promise ('! α)))).
+                                 (tele_app (λ α, 𝟙 -{ coop }-∘ ! α)) (tele_app (λ α, Promise (! α)))).
     iApply sem_typed_var'.
   Qed.
 
   Lemma await_typed :
-    ⊢ ⊨ᵥ await : (∀T: α, Promise ('! α) -{ coop }-> '! α).
+    ⊢ ⊨ᵥ await : (∀ₜ α, Promise (! α) -{ coop }-> ! α).
   Proof.
     rewrite /await. iIntros.
     iApply sem_typed_Tclosure. iIntros (α).
-    iApply sem_typed_closure; solve_sidecond. simpl.
+    smart_apply sem_typed_closure. simpl.
     iApply sem_typed_sub_row; first iApply row_le_rec_fold.
     rewrite /coop_pre -/coop. 
     iApply sem_typed_sub_row; first iApply row_le_swap_second; first done.
     iApply (sem_typed_perform_os (TT:=[tele _]) [tele_arg (α : sem_ty Σ)] _ "await" 
-                                 (tele_app (λ α, Promise ('! α))) (tele_app (λ α, '! α))).
+                                 (tele_app (λ α, Promise (! α))) (tele_app (λ α, ! α))).
     iApply sem_typed_var'.
   Qed.
 
   Lemma yield_typed :
     ⊢ ⊨ᵥ yield : ( 𝟙 -{ coop }-> 𝟙 ).
   Proof.
-    iIntros. iApply sem_typed_closure; try done. simpl.
-    iApply (sem_typed_app_os (Promise ('! 𝟙))).
+    iIntros. iApply sem_typed_closure; first done. simpl.
+    iApply (sem_typed_app_os (Promise (! 𝟙))).
     - iApply sem_typed_sub_u2aarr.
       iApply sem_typed_sub_ty; [iApply ty_le_uarr|]; 
         [iApply row_le_refl|iApply ty_le_refl|iApply (ty_le_mbang_elim MS)|].
       iApply sem_typed_sub_nil. simpl. rewrite -/coop.
-      set C := (λ α, (Promise ('! α)) -{ coop }-> ('! α)).
-      rewrite -/(C 𝟙). iApply sem_typed_TApp; first solve_copy.
+      set C := (λ α, (Promise (! α)) -{ coop }-> (! α)).
+      rewrite -/(C 𝟙). iApply sem_typed_TApp.
       iApply sem_typed_val. iApply await_typed.
-    - iApply (sem_typed_app_os (𝟙 -{ coop }-∘ '! 𝟙)).
+    - iApply (sem_typed_app_os (𝟙 -{ coop }-∘ ! 𝟙)).
       + iApply sem_typed_sub_nil. iApply sem_typed_sub_u2aarr.
-        set C := (λ α, (𝟙 -{ coop }-∘ '! α) -{ coop }-> Promise ('! α)).
-        rewrite -/(C 𝟙). iApply sem_typed_TApp; first solve_copy.
+        set C := (λ α, (𝟙 -{ coop }-∘ ! α) -{ coop }-> Promise (! α)).
+        rewrite -/(C 𝟙). iApply sem_typed_TApp.
         iApply sem_typed_val. iApply async_typed.
       + iApply sem_typed_sub_nil.
         rewrite - {1} (app_nil_r []).
-        iApply sem_typed_afun; solve_sidecond. simpl.
-        iApply sem_typed_sub_ty; [iApply (ty_le_mbang_intro MS); solve_copy|].
+        smart_apply sem_typed_afun. simpl.
+        iApply sem_typed_sub_ty; [iApply (ty_le_mbang_intro_unit)|].
         iApply sem_typed_unit'.
   Qed.
 
@@ -244,18 +235,18 @@ Section typing.
     ⊢ ⊨ᵥ iter : iter_ty τ.
   Proof.
     iApply sem_typed_Rclosure. iIntros (σ).
-    iApply sem_typed_closure; solve_sidecond. simpl.
+    iApply sem_typed_closure; first done. simpl.
     rewrite - [[("g", _); ("f", _)]]app_nil_r. 
-    iApply sem_typed_afun; solve_sidecond. simpl.
+    smart_apply sem_typed_afun. simpl.
     set Γ₂ := [("g", τ -{ ¡ σ }-> 𝟙);
                ("f", ((τ -{ ¡ σ }-> 𝟙) → List τ -{ ¡ σ }-∘ 𝟙)%T)].
-    iApply (sem_typed_match_list _ _ _ _ Γ₂); solve_sidecond.
+    smart_apply (sem_typed_match_list _ _ _ _ Γ₂).
     - iApply sem_typed_var'.
     - do 2 iApply sem_typed_weaken. iApply sem_typed_unit'.
     - iApply sem_typed_seq.
       + iApply sem_typed_swap_third. iApply sem_typed_swap_second. 
         iApply sem_typed_app_os; [|iApply sem_typed_var'].
-        iApply sem_typed_contraction; solve_sidecond.
+        iApply sem_typed_contraction.
         simpl. iApply sem_typed_sub_u2aarr.
         iApply sem_typed_var'.
       + iApply sem_typed_swap_second. rewrite -/Γ₂.
@@ -271,9 +262,9 @@ Section typing.
     ⊢ ⊨ᵥ add : (Queue → add_ty).
   Proof.
     iIntros. rewrite /add_ty.
-    iApply sem_typed_closure; solve_sidecond. simpl.
+    iApply sem_typed_closure; first done. simpl.
     set q := ("q", Queue). rewrite -(app_nil_r [q]).
-    iApply sem_typed_ufun; solve_sidecond. simpl.
+    smart_apply sem_typed_ufun. simpl.
     set f := ("f", 𝟙 ⊸ 𝟙).
     iApply sem_typed_seq; [|iApply sem_typed_unit].
     iApply sem_typed_replace_cpy_os; [iApply sem_typed_var|].
@@ -281,7 +272,7 @@ Section typing.
     { iApply sem_typed_swap_second. iApply sem_typed_var. }
     iApply sem_typed_swap_second.
     iApply sem_typed_replace_cpy_os; [|iApply sem_typed_nil].
-    iApply sem_typed_contraction; solve_sidecond.
+    iApply sem_typed_contraction.
     iApply sem_typed_var.
   Qed.
 
@@ -289,12 +280,12 @@ Section typing.
     ⊢ ⊨ᵥ next : (Queue → next_ty).
   Proof.
     iIntros. rewrite /next_ty.
-    iApply sem_typed_closure; solve_sidecond. simpl.
+    iApply sem_typed_closure; first done. simpl.
     set q := ("q", Queue). rewrite -(app_nil_r [q]).
-    iApply sem_typed_ufun; solve_sidecond. simpl.
-    iApply (sem_typed_match_list _ _ _ _ [q]); solve_sidecond.
+    smart_apply sem_typed_ufun. simpl.
+    smart_apply (sem_typed_match_list _ _ _ _ [q]).
     - iApply sem_typed_replace_cpy_os; [|iApply sem_typed_nil].
-      iApply sem_typed_contraction; solve_sidecond.
+      iApply sem_typed_contraction.
       iApply sem_typed_var.
     - iApply sem_typed_weaken. iApply sem_typed_unit.
     - iApply sem_typed_swap_second.
@@ -312,21 +303,21 @@ Section typing.
     ⊢ ⊨ᵥ resume_task : (add_ty → resume_task_ty).
   Proof.
     iIntros. rewrite /resume_task_ty.
-    iApply sem_typed_closure; solve_sidecond. simpl.
+    iApply sem_typed_closure; first done. simpl.
     set add := ("add", add_ty)%T. rewrite -(app_nil_r [add]).
     iApply sem_typed_oval.
-    iApply sem_typed_TLam; solve_sidecond. 
+    iApply sem_typed_TLam.
     iIntros (α).
     rewrite -(app_nil_r [add]).
-    iApply sem_oval_typed_ufun; solve_sidecond. simpl.
-    rewrite -(app_nil_r [("v", '! α); add]).
-    set v := ("v", '! α).
-    iApply sem_typed_ufun; solve_sidecond. simpl.
-    set k := ("k", '! α ⊸ 𝟙).
+    smart_apply sem_oval_typed_ufun. simpl.
+    rewrite -(app_nil_r [("v", ! α); add]).
+    set v := ("v", ! α).
+    smart_apply sem_typed_ufun. simpl.
+    set k := ("k", ! α ⊸ 𝟙).
     iApply sem_typed_app_os.
     { iApply sem_typed_sub_u2aarr. iApply sem_typed_var. }
     replace ([k; v; add]) with ([k;v] ++ [add]) by done.
-    iApply sem_typed_afun; solve_sidecond. simpl.
+    smart_apply sem_typed_afun. simpl.
     iApply sem_typed_swap_second.
     iApply sem_typed_app_os; iApply sem_typed_var.
   Qed.
@@ -335,54 +326,50 @@ Section typing.
     ⊢ ⊨ᵥ runner : runner_ty.
   Proof.
     iIntros. iApply sem_typed_Tclosure. iIntros (α).
-    iApply sem_typed_closure; solve_sidecond. simpl.
-    set main := ("main", 𝟙 -{ coop }-∘ '! α).
-    iApply (sem_typed_let _ _ _ _  [main]); solve_sidecond.
+    iApply sem_typed_closure; first done. simpl.
+    set main := ("main", 𝟙 -{ coop }-∘ ! α).
+    smart_apply (sem_typed_let _ _ _ _  [main]).
     { iApply (sem_typed_alloc_cpy (List (𝟙 ⊸ 𝟙))). iApply sem_typed_nil. }
-    iApply sem_typed_contraction; solve_sidecond.
+    iApply sem_typed_contraction.
     set q := ("q", Queue).
-    iApply (sem_typed_let _ _ _ _ [q; main]); solve_sidecond.
+    smart_apply (sem_typed_let _ _ _ _ [q; main]).
     { iApply sem_typed_app_os; [|iApply sem_typed_var].
       iApply sem_typed_sub_u2aarr.
       iApply sem_typed_val. iApply add_typed. }
     set add := ("add", add_ty).
     iApply sem_typed_swap_second. 
-    iApply (sem_typed_let _ _ _ _ [add; main]); solve_sidecond. 
+    smart_apply (sem_typed_let _ _ _ _ [add; main]). 
     { rewrite /next. iApply sem_typed_app_os; [|iApply sem_typed_var].
       iApply sem_typed_sub_u2aarr.
       iApply sem_typed_val. iApply next_typed. }
     set next := ("next", next_ty).
     iApply sem_typed_swap_second. 
-    iApply sem_typed_contraction; solve_sidecond.
-    iApply (sem_typed_let _ _ _ _ [add; next; main]); solve_sidecond.
+    iApply sem_typed_contraction.
+    smart_apply (sem_typed_let _ _ _ _ [add; next; main]).
     { iApply sem_typed_app_os; [|iApply sem_typed_var].
       iApply sem_typed_sub_u2aarr.
       iApply sem_typed_val. iApply resume_task_typed. }
     set resume_task := ("resume_task", resume_task_ty).
     rewrite -/next -/resume_task -/add.
-    iApply (sem_typed_let _ _ _ _ [main]); solve_sidecond.
+    smart_apply (sem_typed_let _ _ _ _ [main]).
     - assert (Hrw : [resume_task;add;next;main] = [resume_task;add;next] ++ [main]) by done.
       rewrite Hrw. clear Hrw. iApply sem_typed_oval.
-      iApply (sem_typed_ufun_poly_rec (λ β, Promise ('! β)) (λ _, ⊥) (λ β, (𝟙 -{ coop }-∘ '! β) ⊸ 𝟙)); 
-        solve_sidecond.
-      { iIntros. iApply copy_ty_uarr. }
+      smart_apply (sem_typed_ufun_poly_rec (λ β, Promise (! β)) (λ _, ⊥) (λ β, (𝟙 -{ coop }-∘ ! β) ⊸ 𝟙)).
      simpl. iIntros (β) "/=". 
-     set promise := ("promise", Promise ('! β)).
-     set fulfill := ("fulfill", ∀T: β', Promise ('! β') → (𝟙 -{ coop }-∘ '! β') ⊸ 𝟙).
+     set promise := ("promise", Promise (! β)).
+     set fulfill := ("fulfill", ∀ₜ β', Promise (! β') → (𝟙 -{ coop }-∘ ! β') ⊸ 𝟙).
      rewrite -(app_nil_r [promise;fulfill;resume_task;add;next]).
-     iApply sem_typed_afun; solve_sidecond. simpl.
-     set comp := ("comp", 𝟙 -{ coop }-∘ '! β)%T.
+     smart_apply sem_typed_afun. simpl.
+     set comp := ("comp", 𝟙 -{ coop }-∘ ! β)%T.
      replace ([comp; promise; fulfill; resume_task; add;next]) with
              ([comp] ++ [promise; fulfill; resume_task; add;next]) by done.
-     iApply (sem_typed_handler2 (TT:=[tele _]) OS "async" "await" 
-                    (tele_app (λ α, 𝟙 -{ coop }-∘ '! α)) 
-                    (tele_app (λ α, Promise ('! α))) 
-                    (tele_app (λ α, Promise ('! α))) 
-                    (tele_app (λ α, '! α))  _ _ _ _ [comp] []); solve_sidecond.
-     + iIntros. iApply copy_ty_uarr.
-     + iIntros. iApply copy_ty_uarr.
+     smart_apply (sem_typed_handler2 (TT:=[tele _]) OS "async" "await" 
+                    (tele_app (λ α, 𝟙 -{ coop }-∘ ! α)) 
+                    (tele_app (λ α, Promise (! α))) 
+                    (tele_app (λ α, Promise (! α))) 
+                    (tele_app (λ α, ! α))  _ _ _ _ [comp] []).
      + iApply row_le_refl.
-     + iApply (sem_typed_app_os 𝟙 _ ('! β)); [iApply sem_typed_var'|]. 
+     + iApply (sem_typed_app_os 𝟙 _ (! β)); [iApply sem_typed_var'|]. 
        rewrite -/await_sig -/(async_sig coop) -/coop. 
        iApply sem_typed_sub_env_final; first iApply env_le_cons; first iApply env_le_refl; 
        [iApply ty_le_arr; try iApply ty_le_refl; iApply (row_le_rec_unfold coop_pre)|].
@@ -390,48 +377,48 @@ Section typing.
      + iIntros (β').
        iApply sem_typed_swap_third. iApply sem_typed_weaken.
        iApply sem_typed_swap_fourth. iApply sem_typed_weaken.
-       set x := ("x", 𝟙 -{ coop }-∘ '! β').
-       set k := ("k", Promise ('!β') ⊸ 𝟙).
+       set x := ("x", 𝟙 -{ coop }-∘ ! β').
+       set k := ("k", Promise (!β') ⊸ 𝟙).
        rewrite -/x -/k -/fulfill -/add -/next.
-       iApply (sem_typed_let (Promise ('! β')) _ _ _ [x;k;fulfill;add;next]); solve_sidecond. 
+       smart_apply (sem_typed_let (Promise (! β')) _ _ _ [x;k;fulfill;add;next]).
        { iApply sem_typed_alloc_cpy. iApply sem_typed_right_inj. iApply sem_typed_nil. }
-       set new_prom := ("new_prom", Promise ('! β')). 
+       set new_prom := ("new_prom", Promise (! β')). 
        iApply (sem_typed_seq _ _ _ _ [new_prom; k; next]).
        * iApply (sem_typed_app_os (𝟙 ⊸ 𝟙)%T _ 𝟙 _ [new_prom; k; add; next]).
          { iApply sem_typed_swap_third. iApply sem_typed_sub_u2aarr. iApply sem_typed_var'. }
          iApply sem_typed_swap_fourth. iApply sem_typed_swap_second.
-         iApply sem_typed_contraction; solve_sidecond.
+         iApply sem_typed_contraction.
          do 2 iApply sem_typed_swap_fourth.
          assert (Hrw : [fulfill; x; new_prom; new_prom; k; add; next] = 
                        [fulfill; x; new_prom] ++ [new_prom; k; add; next]) by done.
          rewrite Hrw. clear Hrw.
-         iApply sem_typed_afun; solve_sidecond. simpl.
+         smart_apply sem_typed_afun. simpl.
          do 2 (iApply sem_typed_swap_second; iApply sem_typed_app_os; [|iApply sem_typed_var]).
-         set C := (λ β, Promise ('! β) → (𝟙 -{ coop }-∘ '! β) ⊸ 𝟙)%T.
+         set C := (λ β, Promise (! β) → (𝟙 -{ coop }-∘ ! β) ⊸ 𝟙)%T.
          iApply sem_typed_sub_u2aarr. rewrite -/(C β').
-         iApply sem_typed_TApp; first solve_copy. iApply sem_typed_var.
+         iApply sem_typed_TApp. iApply sem_typed_var.
       * simpl.
         iApply sem_typed_swap_third. iApply sem_typed_weaken.
         iApply sem_typed_app_os; iApply sem_typed_var'.
      + iIntros (β').
-       set x := ("x", Promise ('! β')).
-       set k := ("k", '! β' ⊸ 𝟙).
+       set x := ("x", Promise (! β')).
+       set k := ("k", ! β' ⊸ 𝟙).
        do 4 (iApply sem_typed_swap_third; iApply sem_typed_weaken).
-       iApply (sem_typed_match ('! β') _ _  _ _ [x;k;next]); solve_sidecond.
+       smart_apply (sem_typed_match (! β') _ _  _ _ [x;k;next]).
        * iApply sem_typed_replace_cpy_os; first iApply sem_typed_var.
-         iApply sem_typed_contraction; solve_sidecond.
+         iApply sem_typed_contraction.
          iApply sem_typed_right_inj. iApply sem_typed_nil.
-       * simpl. set v := ("v", '! β').
+       * simpl. set v := ("v", ! β').
          iApply sem_typed_swap_fourth. iApply sem_typed_weaken.
-         iApply sem_typed_contraction; solve_sidecond.
+         iApply sem_typed_contraction.
          iApply sem_typed_swap_third. iApply sem_typed_swap_second.
          iApply (sem_typed_seq _ _ _ _ [v; k]).
          { iApply sem_typed_replace_cpy_os; [iApply sem_typed_var|].
            iApply sem_typed_left_inj. iApply sem_typed_var. }
          iApply sem_typed_app_os; [iApply sem_typed_var|].
          iApply sem_typed_var.
-       * simpl. set ks := ("ks", List ('! β' ⊸ 𝟙)).
-         iApply (sem_typed_seq (Status ('! β'))).
+       * simpl. set ks := ("ks", List (! β' ⊸ 𝟙)).
+         iApply (sem_typed_seq (Status (! β'))).
          ** iApply sem_typed_swap_third. 
             iApply sem_typed_replace_cpy_os; first iApply sem_typed_var.
             iApply sem_typed_right_inj. 
@@ -446,19 +433,19 @@ Section typing.
       iApply sem_typed_swap_third. iApply sem_typed_weaken.
       iApply sem_typed_swap_fourth; iApply sem_typed_weaken.
       iApply sem_typed_swap_second.
-      set x := ("x", '!β). rewrite -/resume_task -/promise.
-      iApply (sem_typed_let _ _ _ _ [promise; x; resume_task; next]); solve_sidecond.
+      set x := ("x", !β). rewrite -/resume_task -/promise.
+      smart_apply (sem_typed_let _ _ _ _ [promise; x; resume_task; next]).
       * iApply sem_typed_replace_cpy_os; [|iApply sem_typed_right_inj; iApply sem_typed_nil].
-        iApply sem_typed_contraction; solve_sidecond.
+        iApply sem_typed_contraction.
         iApply sem_typed_var.
-      * set v := ("v", '! β + (List ('! β ⊸ 𝟙))).
-        iApply (sem_typed_match  _ _ _ _ _ [promise; x; resume_task; next]); solve_sidecond;
+      * set v := ("v", ! β + (List (! β ⊸ 𝟙))).
+        smart_apply (sem_typed_match  _ _ _ _ _ [promise; x; resume_task; next]);
           [iApply sem_typed_var| |].
         { simpl. do 4 (iApply sem_typed_weaken). iApply impossible_typed. }
         simpl. iApply sem_typed_swap_second. 
-        iApply sem_typed_swap_third. iApply sem_typed_contraction; solve_sidecond.
+        iApply sem_typed_swap_third. iApply sem_typed_contraction.
         iApply sem_typed_swap_third. iApply sem_typed_swap_second.
-        set ks := ("ks", List ('! β ⊸ 𝟙)).
+        set ks := ("ks", List (! β ⊸ 𝟙)).
         iApply (sem_typed_seq _ _ _ _ [x; ks; resume_task; next]).
         ** iApply sem_typed_replace_cpy_os; [iApply sem_typed_var|].
            iApply sem_typed_left_inj. iApply sem_typed_var.
@@ -467,37 +454,37 @@ Section typing.
                 iApply sem_typed_sub_u2aarr; iApply sem_typed_var. }
            iApply sem_typed_swap_second.
            iApply sem_typed_app_os; [|iApply sem_typed_var].
-           iApply (sem_typed_app_os (('! β ⊸ 𝟙) → 𝟙)%T).
+           iApply (sem_typed_app_os ((! β ⊸ 𝟙) → 𝟙)%T).
            2: { iApply sem_typed_app_os; [|iApply sem_typed_var]. 
                 iApply sem_typed_sub_u2aarr.
-                set C := λ β, ('! β → ('! β ⊸ 𝟙) → 𝟙)%T. rewrite -/(C β). simpl.
-                iApply sem_typed_TApp; first solve_sidecond. iApply sem_typed_var. }
+                set C := λ β, (! β → (! β ⊸ 𝟙) → 𝟙)%T. rewrite -/(C β). simpl.
+                iApply sem_typed_TApp. iApply sem_typed_var. }
            iApply sem_typed_sub_u2aarr.
            iApply sem_typed_sub_ty; first iApply ty_le_uarr; 
             [iApply row_le_refl|iApply ty_le_uarr|iApply ty_le_refl|];
             [iApply (row_le_mfbang_intro OS)|iApply ty_le_refl|iApply ty_le_refl|].
            iApply sem_typed_sub_ty; first iApply ty_le_uarr; 
             [iApply row_le_refl|iApply ty_le_refl|iApply ty_le_arr|];
-            [iApply (row_le_mfbang_elim OS)|iApply ty_le_refl|iApply ty_le_refl|].
-           set C := (λ (θ : sem_row Σ), (('! β ⊸ 𝟙) -{ ¡ θ }-> 𝟙) → List ('! β ⊸ 𝟙) -{ ¡ θ }-∘ 𝟙)%T.
+            [iApply (@row_le_mfbang_elim _ _ )|iApply ty_le_refl|iApply ty_le_refl|].
+           set C := (λ (θ : sem_row Σ), ((! β ⊸ 𝟙) -{ ¡ θ }-> 𝟙) → List (! β ⊸ 𝟙) -{ ¡ θ }-∘ 𝟙)%T.
            rewrite -/(C ⊥).
-           iApply sem_typed_RApp; first solve_copy. 
+           iApply sem_typed_RApp.
            iApply sem_typed_val. iApply iter_typed.
-  - set fulfill := ("fulfill", ∀T: α, Promise ('! α) → (𝟙 -{ coop }-∘ '! α) ⊸ 𝟙).
-    iApply (sem_typed_let _ _ _ _ [fulfill; main]); solve_sidecond.
-    { iApply (sem_typed_alloc_cpy (Status ('! α))). 
+  - set fulfill := ("fulfill", ∀ₜ α, Promise (! α) → (𝟙 -{ coop }-∘ ! α) ⊸ 𝟙).
+    smart_apply (sem_typed_let _ _ _ _ [fulfill; main]).
+    { iApply (sem_typed_alloc_cpy (Status (! α))). 
       iApply sem_typed_right_inj. iApply sem_typed_nil. }
-    set pmain := ("pmain", Refᶜ Status ('! α)).
-    iApply sem_typed_contraction; solve_sidecond.
+    set pmain := ("pmain", Refᶜ Status (! α)).
+    iApply sem_typed_contraction.
     iApply sem_typed_swap_third. iApply sem_typed_swap_second. iApply sem_typed_swap_fourth.
     iApply (sem_typed_seq 𝟙).
     + do 2 (iApply sem_typed_app_os; [|iApply sem_typed_var]). 
       iApply sem_typed_sub_u2aarr. 
-      set C := (λ α, Promise ('! α) → (𝟙 -{ coop }-∘ '! α) ⊸ 𝟙)%T.
+      set C := (λ α, Promise (! α) → (𝟙 -{ coop }-∘ ! α) ⊸ 𝟙)%T.
       rewrite -/(C α).
       iApply sem_typed_TApp. rewrite /C /Promise.
       iApply sem_typed_var.
-    + iApply (sem_typed_match _ _ _ _ _ []); solve_sidecond; simpl; [|iApply sem_typed_var|].
+    + smart_apply (sem_typed_match _ _ _ _ _ []); simpl; [|iApply sem_typed_var|].
       { iApply sem_typed_replace_cpy_os; [iApply sem_typed_var|].
         iApply sem_typed_right_inj. iApply sem_typed_nil. }
       iApply impossible_typed. 
