theories/case_studies/cooperative_concurrency_gen.v
@@ -29,9 +29,9 @@ From affect.case_studies Require Import state.
 
 (* Make all the definitions opaque so that we do not rely on their definition in the model to show that the programs are well-typed terms. *)
 Opaque sem_typed sem_typed_val ty_le row_le sig_le row_type_sub row_env_sub.
-Opaque sem_ty_void sem_ty_unit sem_ty_bool sem_ty_int sem_ty_string sem_ty_top sem_ty_bang sem_env_bang sem_ty_ref_cpy sem_ty_ref sem_ty_prod sem_ty_sum sem_ty_arr sem_ty_forall sem_ty_row_forall sem_ty_exists sem_ty_rec sem_ty_option sem_ty_list.
-Opaque sem_sig_eff sem_sig_flip_bang.
-Opaque sem_row_nil sem_row_flip_bang sem_row_cons sem_row_rec.
+Opaque sem_ty_bot sem_ty_unit sem_ty_bool sem_ty_int sem_ty_string sem_ty_top sem_ty_mbang env_mbang sem_ty_ref_cpy sem_ty_ref sem_ty_prod sem_ty_sum sem_ty_arr sem_ty_type_forall sem_ty_row_forall sem_ty_exists sem_ty_rec sem_ty_option.
+Opaque sem_sig_eff sem_sig_flip_mbang.
+Opaque sem_row_nil sem_row_flip_mbang sem_row_cons sem_row_rec.
 
 Definition impossible : expr := ((rec: "f" <> := "f" #()) #())%E.
 
@@ -114,16 +114,16 @@ Section typing.
 
   Context `{!heapGS Σ}.
 
-  Definition Queue θ' := Refᶜ (List (() -{ θ' }-∘ ())).
+  Definition Queue θ' := Refᶜ (List (𝟙 -{ θ' }-∘ 𝟙)).
 
-  Definition Status τ θ' := τ + List (τ -{ θ' }-∘ ()).
+  Definition Status τ θ' := τ + List (τ -{ θ' }-∘ 𝟙).
 
   Definition Promise τ θ' := Refᶜ (Status τ θ').
 
-  Definition await_sig θ' : sem_sig Σ := (∀S: α, Promise ('! α) θ' =[ OS ]=> '! α)%S.
+  Definition await_sig θ' : sem_sig Σ := (∀ₛ α, Promise (! α) θ' =[ OS ]=> ! α)%S.
 
   Definition async_sig (θ' θ : sem_row Σ) : sem_sig Σ := 
-    (∀S: α, ( () -{ θ }-∘ '! α ) =[ OS ]=> Promise ('! α) θ')%S. 
+    (∀ₛ α, ( 𝟙 -{ θ }-∘ ! α ) =[ OS ]=> Promise (! α) θ')%S. 
 
   Definition coop_pre (θ' θ : sem_row Σ) : sem_row Σ := 
     (("async", async_sig θ' θ) · ("await", await_sig θ') · θ')%R.
@@ -131,141 +131,130 @@ Section typing.
   Local Instance promise_ne τ :
     NonExpansive (Promise τ).
   Proof.
-    intros ?????. rewrite /Promise. apply non_dep_fun_dist.
-    f_equiv. rewrite /Status. by do 3 f_equiv.
+    rewrite /Promise /Status. 
+    intros ????. by repeat f_equiv.
   Qed.
 
   Local Instance await_arg_sig_ne θ' :
-    NonExpansive (λ (α : sem_ty Σ), Promise ('! α) θ').
+    NonExpansive (λ (α : sem_ty Σ), Promise (! α) θ').
   Proof.
-    rewrite /Promise /Status. intros ?????.
-    apply non_dep_fun_dist. by repeat f_equiv.
+    rewrite /Promise /Status. 
+    intros ????. by repeat f_equiv.
   Qed.
 
   Local Instance await_res_sig_ne :
-    NonExpansive
-      (λ (α : sem_ty Σ), '! α).
-  Proof.
-    intros ????. by repeat f_equiv.
-  Qed.
+    NonExpansive (λ (α : sem_ty Σ), ! α).
+  Proof. intros ????. by repeat f_equiv. Qed.
 
   Local Instance await_sig_ne :
     NonExpansive await_sig.
   Proof.
     rewrite /await_sig. intros ????. 
-    apply non_dep_fun_dist. f_equiv.
-    rewrite /tele_app; intros ?; destruct x0. by f_equiv.
+    f_equiv. rewrite /tele_app. intros []; simpl; apply non_dep_fun_dist;
+    repeat f_equiv; intros ?; by repeat f_equiv.
   Qed.
 
   Local Instance async_arg_sig_ne θ :
-    NonExpansive
-      (λ (α : sem_ty Σ), () -{ θ }-∘ '! α).
-  Proof.
-    intros ?????. apply non_dep_fun_dist.
-    do 2 f_equiv; try done. 
-  Qed.
+    NonExpansive (λ (α : sem_ty Σ), 𝟙 -{ θ }-∘ ! α).
+  Proof. intros ????. by repeat f_equiv. Qed.
 
   Local Instance async_sig_ne θ' : NonExpansive (async_sig θ').
   Proof.
-    intros ????. rewrite /async_sig. f_equiv;
-    rewrite /tele_app; intros ?; destruct x0; by f_equiv.
+    rewrite /async_sig. 
+    intros ????. 
+    f_equiv. rewrite /tele_app. intros []; simpl; apply non_dep_fun_dist;
+    repeat f_equiv; intros ?; by repeat f_equiv.
   Qed.
 
   Local Instance contractive_coop_pre θ' : Contractive (coop_pre θ').
   Proof. 
-    intros ????. rewrite /coop_pre. f_equiv. f_equiv. f_equiv. 
+    intros ????. rewrite /coop_pre. do 3 f_equiv.
     destruct n; first apply dist_later_0.
     apply dist_later_S. rewrite - dist_later_S in H.
     by f_equiv. 
   Qed.
 
-  Definition coop θ' : sem_row Σ := (μR: θ, coop_pre θ' θ)%R.
+  Definition coop θ' : sem_row Σ := (μᵣ θ, coop_pre θ' θ)%R.
 
-  Local Instance coop_os_row (θ' : sem_row Σ) `{Once θ'} : Once (coop θ').
-  Proof.
-    rewrite /coop. apply row_rec_once. iIntros (θ).
-    rewrite /coop_pre. apply row_cons_once.
-    { rewrite /async_sig. apply sig_eff_os_once; apply _. }
-    apply row_cons_once; last apply _.
-    apply sig_eff_os_once; apply _.
-  Qed.
+  Local Instance coop_os_row (θ' : sem_row Σ) `{! OnceR θ'} : OnceR (coop θ').
+  Proof. apply _. Qed.
 
-  Definition iter_ty τ := (∀R: θ, (τ -{ ¡ θ }-> ()) → List τ -{ ¡ θ }-∘ ())%T.
+  Definition iter_ty τ := (∀ᵣ θ, (τ -{ ¡ θ }-> 𝟙) → List τ -{ ¡ θ }-∘ 𝟙)%T.
   
-  Definition next_ty θ' := (() -{ θ' }-> ())%T.
+  Definition next_ty θ' := (𝟙 -{ θ' }-> 𝟙)%T.
 
-  Definition add_ty θ' := ((() -{ θ' }-∘ ()) → ())%T.
+  Definition add_ty θ' := ((𝟙 -{ θ' }-∘ 𝟙) → 𝟙)%T.
 
-  Definition resume_task_ty θ' := (∀T: α, '! α → ('! α -{ θ' }-∘ ()) → ())%T.
+  Definition resume_task_ty θ' := (∀ₜ α, ! α → (! α -{ θ' }-∘ 𝟙) → 𝟙)%T.
   
-  Definition runner_ty := (∀T: α, ∀R: θ', (() -{ coop θ' }-∘ '! α) -{ θ' }-> '! α)%T.
+  Definition runner_ty := (∀ₜ α, ∀ᵣ θ', (𝟙 -{ coop θ' }-∘ ! α) -{ θ' }-> ! α)%T.
 
   Lemma impossible_typed τ :
-    ⊢ ⊨ impossible : ⊥ : τ.
+    ⊢ ⊨ impossible : ⟨⟩ : τ.
   Proof.
     iIntros. rewrite /impossible.
     iApply sem_typed_app_os; [|iApply sem_typed_unit].
     rewrite - {1} (app_nil_r []).
     iApply sem_typed_sub_u2aarr.
-    iApply sem_typed_ufun; solve_sidecond. simpl.
+    smart_apply sem_typed_ufun. simpl.
     iApply sem_typed_app_os; [|iApply sem_typed_unit].
     iApply sem_typed_sub_u2aarr.
     iApply sem_typed_var.
   Qed.
 
   Lemma async_typed :
-    ⊢ ⊨ᵥ async : (∀R: θ', ∀T: α, (() -{ coop θ' }-∘ '! α) -{ coop θ' }-> Promise ('! α) θ').
+    ⊢ ⊨ᵥ async : (∀ᵣ θ', ∀ₜ α, (𝟙 -{ coop θ' }-∘ ! α) -{ coop θ' }-> Promise (! α) θ').
   Proof.
     rewrite /async. iIntros.
     iApply sem_typed_Rclosure. iIntros (θ').
-    iApply sem_typed_Tclosure; first solve_copy. iIntros (α).
-    iApply sem_typed_closure; solve_sidecond. simpl. rewrite {2} /coop.
+    iApply sem_typed_Tclosure. iIntros (α).
+    iApply sem_typed_closure; first done. simpl. rewrite {2} /coop.
     iApply sem_typed_sub_row; first iApply row_le_rec_fold.
     rewrite - {1} /(coop θ') {1} /coop_pre. 
     iApply (sem_typed_perform_os (TT:=[tele _]) [tele_arg (α : sem_ty Σ)] _ "async"
-                                 (tele_app (λ α, () -{ coop θ' }-∘ '! α)) (tele_app (λ α, Promise ('! α) θ'))).
+                                 (tele_app (λ α, 𝟙 -{ coop θ' }-∘ ! α)) (tele_app (λ α, Promise (! α) θ'))).
     iApply sem_typed_var'.
   Qed.
 
   Lemma await_typed :
-    ⊢ ⊨ᵥ await : (∀R: θ', ∀T: α, Promise ('! α) θ' -{ coop θ' }-> '! α).
+    ⊢ ⊨ᵥ await : (∀ᵣ θ', ∀ₜ α, Promise (! α) θ' -{ coop θ' }-> ! α).
   Proof.
     rewrite /await. iIntros.
     iApply sem_typed_Rclosure. iIntros (θ').
-    iApply sem_typed_Tclosure; first solve_copy. iIntros (α).
-    iApply sem_typed_closure; solve_sidecond. simpl.
+    iApply sem_typed_Tclosure. iIntros (α).
+    iApply sem_typed_closure; first done. simpl.
     iApply sem_typed_sub_row; first iApply row_le_rec_fold.
     rewrite - {1} /(coop θ') {1} /coop_pre. 
     iApply sem_typed_sub_row; first iApply row_le_swap_second; first done.
     iApply (sem_typed_perform_os (TT:=[tele _]) [tele_arg (α : sem_ty Σ)] _ "await" 
-                                 (tele_app (λ α, Promise ('! α) θ')) (tele_app (λ α, '! α))).
+                                 (tele_app (λ α, Promise (! α) θ')) (tele_app (λ α, ! α))).
     iApply sem_typed_var'.
   Qed.
 
   Lemma yield_typed :
-    ⊢ ⊨ᵥ yield : ( () -{ coop ⟨⟩ }-> () ).
+    ⊢ ⊨ᵥ yield : ( 𝟙 -{ coop ⟨⟩ }-> 𝟙 ).
   Proof.
-    iIntros. iApply sem_typed_closure; try done. simpl.
-    iApply (sem_typed_app_os (Promise ('! ()) ⟨⟩%R)).
+    iIntros. iApply sem_typed_closure; first done. simpl.
+    iApply (sem_typed_app_os (Promise (! 𝟙) ⟨⟩%R)).
     - iApply sem_typed_sub_u2aarr.
       iApply sem_typed_sub_ty; [iApply ty_le_uarr|]; 
         [iApply row_le_refl|iApply ty_le_refl|iApply (ty_le_mbang_elim MS)|].
       iApply sem_typed_sub_nil. simpl. rewrite -/coop.
-      set C := (λ θ' α, (Promise ('! α) θ') -{ coop θ' }-> ('! α)).
-      rewrite -/(C ⟨⟩%R ()). iApply sem_typed_TApp; first solve_copy.
-      set D := (λ ρ, ∀T: α, C ρ α)%T.
-      iApply (sem_typed_RApp D); first solve_copy.
+      set C := (λ θ' α, (Promise (! α) θ') -{ coop θ' }-> (! α)).
+      rewrite -/(C ⟨⟩%R 𝟙). iApply sem_typed_TApp.
+      set D := (λ ρ, ∀ₜ α, C ρ α)%T.
+      iApply (sem_typed_RApp D).
       iApply sem_typed_val. iApply await_typed.
-    - iApply (sem_typed_app_os (() -{ coop ⟨⟩ }-∘ '! ())).
+    - iApply (sem_typed_app_os (𝟙 -{ coop ⟨⟩ }-∘ ! 𝟙)).
       + iApply sem_typed_sub_nil. iApply sem_typed_sub_u2aarr.
-        set C := (λ θ' α, (() -{ coop θ' }-∘ '! α) -{ coop θ' }-> Promise ('! α) θ').
-        rewrite -/(C ⟨⟩%R ()). iApply sem_typed_TApp.
-        set D := (λ ρ, ∀T: α, C ρ α)%T.
+        set C := (λ θ' α, (𝟙 -{ coop θ' }-∘ ! α) -{ coop θ' }-> Promise (! α) θ').
+        rewrite -/(C ⟨⟩%R 𝟙). iApply sem_typed_TApp.
+        set D := (λ ρ, ∀ₜ α, C ρ α)%T.
         iApply (sem_typed_RApp D). iApply sem_typed_val. iApply async_typed.
       + iApply sem_typed_sub_nil.
         rewrite - {1} (app_nil_r []).
-        iApply sem_typed_afun; solve_sidecond. simpl.
-        iApply sem_typed_sub_ty; [iApply (ty_le_mbang_intro MS); solve_copy|].
+        smart_apply sem_typed_afun. simpl.
+        iApply sem_typed_sub_ty; [iApply (ty_le_mbang_intro_unit)|].
         iApply sem_typed_unit'.
   Qed.
 
@@ -273,18 +262,18 @@ Section typing.
     ⊢ ⊨ᵥ iter : iter_ty τ.
   Proof.
     iApply sem_typed_Rclosure. iIntros (σ).
-    iApply sem_typed_closure; solve_sidecond. simpl.
+    iApply sem_typed_closure; first done. simpl.
     rewrite - [[("g", _); ("f", _)]]app_nil_r. 
-    iApply sem_typed_afun; solve_sidecond. simpl.
-    set Γ₂ := [("g", τ -{ ¡ σ }-> ());
-               ("f", ((τ -{ ¡ σ }-> ()) → List τ -{ ¡ σ }-∘ ())%T)].
-    iApply (sem_typed_match_list _ _ _ _ Γ₂); solve_sidecond.
+    smart_apply sem_typed_afun. simpl.
+    set Γ₂ := [("g", τ -{ ¡ σ }-> 𝟙);
+               ("f", ((τ -{ ¡ σ }-> 𝟙) → List τ -{ ¡ σ }-∘ 𝟙)%T)].
+    smart_apply (sem_typed_match_list _ _ _ _ Γ₂).
     - iApply sem_typed_var'.
     - do 2 iApply sem_typed_weaken. iApply sem_typed_unit'.
     - iApply sem_typed_seq.
       + iApply sem_typed_swap_third. iApply sem_typed_swap_second. 
         iApply sem_typed_app_os; [|iApply sem_typed_var'].
-        iApply sem_typed_contraction; solve_sidecond.
+        iApply sem_typed_contraction.
         simpl. iApply sem_typed_sub_u2aarr.
         iApply sem_typed_var'.
       + iApply sem_typed_swap_second. rewrite -/Γ₂.
@@ -300,17 +289,17 @@ Section typing.
     ⊢ ⊨ᵥ add : (Queue θ' → add_ty θ').
   Proof.
     iIntros. rewrite /add_ty.
-    iApply sem_typed_closure; solve_sidecond. simpl.
+    iApply sem_typed_closure; first done. simpl.
     set q := ("q", Queue θ'). rewrite -(app_nil_r [q]).
-    iApply sem_typed_ufun; solve_sidecond. simpl.
-    set f := ("f", () -{ θ' }-∘ ()).
+    smart_apply sem_typed_ufun. simpl.
+    set f := ("f", 𝟙 -{ θ' }-∘ 𝟙).
     iApply sem_typed_seq; [|iApply sem_typed_unit].
     iApply sem_typed_replace_cpy_os; [iApply sem_typed_var|].
     iApply sem_typed_cons.
     { iApply sem_typed_swap_second. iApply sem_typed_var. }
     iApply sem_typed_swap_second.
     iApply sem_typed_replace_cpy_os; [|iApply sem_typed_nil].
-    iApply sem_typed_contraction; solve_sidecond.
+    iApply sem_typed_contraction.
     iApply sem_typed_var.
   Qed.
 
@@ -318,110 +307,105 @@ Section typing.
     ⊢ ⊨ᵥ next : (Queue θ' → next_ty θ').
   Proof.
     iIntros. rewrite /next_ty.
-    iApply sem_typed_closure; solve_sidecond. simpl.
+    iApply sem_typed_closure; first done. simpl.
     set q := ("q", Queue θ'). rewrite -(app_nil_r [q]).
-    iApply sem_typed_ufun; solve_sidecond. simpl.
-    iApply (sem_typed_match_list _ _ _ _ [q]); solve_sidecond.
+    smart_apply sem_typed_ufun. simpl.
+    smart_apply (sem_typed_match_list _ _ _ _ [q]).
     - iApply sem_typed_sub_nil.
       iApply sem_typed_replace_cpy_os; [|iApply sem_typed_nil].
-      iApply sem_typed_contraction; solve_sidecond.
+      iApply sem_typed_contraction.
       iApply sem_typed_var.
     - iApply sem_typed_weaken. iApply sem_typed_unit'.
     - iApply sem_typed_swap_second.
       iApply sem_typed_swap_third.
       iApply sem_typed_swap_second.
-      set x := ("x", () -{ θ' }-∘ ()).
-      set xs := ("xs", List (() -{ θ' }-∘ ())).
+      set x := ("x", 𝟙 -{ θ' }-∘ 𝟙).
+      set xs := ("xs", List (𝟙 -{ θ' }-∘ 𝟙)).
       rewrite -/q.
       iApply sem_typed_seq.
       { iApply sem_typed_sub_nil. iApply sem_typed_replace_cpy_os; iApply sem_typed_var. }
-      iApply (sem_typed_app_ms ()); [solve_copy|solve_sidecond|iApply sem_typed_var'|iApply sem_typed_unit'].
+      iApply (sem_typed_app_ms 𝟙); [iApply sem_typed_var'|iApply sem_typed_unit'].
   Qed.
 
   Definition resume_task_typed θ' :
     ⊢ ⊨ᵥ resume_task : (add_ty θ' → resume_task_ty θ').
   Proof.
     iIntros. rewrite /resume_task_ty.
-    iApply sem_typed_closure; solve_sidecond. simpl.
+    iApply sem_typed_closure; first done. simpl.
     set add := ("add", add_ty θ')%T. rewrite -(app_nil_r [add]).
     iApply sem_typed_oval.
-    iApply sem_typed_TLam; solve_sidecond. 
-    iIntros (α).
+    iApply sem_typed_TLam. iIntros (α).
     rewrite -(app_nil_r [add]).
-    iApply sem_oval_typed_ufun; solve_sidecond. simpl.
-    rewrite -(app_nil_r [("v", '! α); add]).
-    set v := ("v", '! α).
-    iApply sem_typed_ufun; solve_sidecond. simpl.
-    set k := ("k", '! α -{ θ' }-∘ ()).
+    smart_apply sem_oval_typed_ufun. simpl.
+    rewrite -(app_nil_r [("v", ! α); add]).
+    set v := ("v", ! α).
+    smart_apply sem_typed_ufun. simpl.
+    set k := ("k", ! α -{ θ' }-∘ 𝟙).
     iApply sem_typed_app_os.
     { iApply sem_typed_sub_u2aarr. iApply sem_typed_var. }
     replace ([k; v; add]) with ([k;v] ++ [add]) by done.
-    iApply sem_typed_afun; solve_sidecond. simpl.
+    smart_apply sem_typed_afun. simpl.
     iApply sem_typed_swap_second.
-    iApply (sem_typed_app_ms ('! α)%T); solve_sidecond; iApply sem_typed_var'.
+    iApply (sem_typed_app_ms (! α)%T); iApply sem_typed_var'.
   Qed.
 
   Definition runner_typed :
     ⊢ ⊨ᵥ runner : runner_ty.
   Proof.
     iIntros. iApply sem_typed_Tclosure. iIntros (α).
-    iApply sem_typed_Rclosure; solve_copy. iIntros (θ').
-    iApply sem_typed_closure; solve_sidecond. simpl.
-    set main := ("main", () -{ coop θ' }-∘ '! α).
-    iApply (sem_typed_let _ _ _ _  [main]); solve_sidecond.
-    { iApply (sem_typed_alloc_cpy (List (() -{ θ' }-∘ ()))). iApply sem_typed_sub_nil. iApply sem_typed_nil. }
-    iApply sem_typed_contraction; solve_sidecond.
+    iApply sem_typed_Rclosure. iIntros (θ').
+    iApply sem_typed_closure; first done. simpl.
+    set main := ("main", 𝟙 -{ coop θ' }-∘ ! α).
+    smart_apply (sem_typed_let _ _ _ _  [main]).
+    { iApply (sem_typed_alloc_cpy (List (𝟙 -{ θ' }-∘ 𝟙))). iApply sem_typed_sub_nil. iApply sem_typed_nil. }
+    iApply sem_typed_contraction.
     set q := ("q", Queue θ').
-    iApply (sem_typed_let _ _ _ _ [q; main]); solve_sidecond.
+    smart_apply (sem_typed_let _ _ _ _ [q; main]).
     { iApply sem_typed_sub_nil.
       iApply sem_typed_app_os; [|iApply sem_typed_var].
       iApply sem_typed_sub_u2aarr.
       iApply sem_typed_val. iApply add_typed. }
     set add := ("add", add_ty θ').
     iApply sem_typed_swap_second. 
-    iApply (sem_typed_let _ _ _ _ [add; main]); solve_sidecond. 
+    smart_apply (sem_typed_let _ _ _ _ [add; main]).
     { iApply sem_typed_sub_nil.
       iApply (sem_typed_app_os (Queue θ')); last iApply sem_typed_var'.
       iApply sem_typed_sub_u2aarr.
       iApply sem_typed_val. iApply next_typed. }
     set next := ("next", next_ty θ').
     iApply sem_typed_swap_second. 
-    iApply sem_typed_contraction; solve_sidecond.
-    iApply (sem_typed_let _ _ _ _ [add; next; main]); solve_sidecond.
+    iApply sem_typed_contraction.
+    smart_apply (sem_typed_let _ _ _ _ [add; next; main]).
     { iApply sem_typed_sub_nil.
       iApply sem_typed_app_os; [|iApply sem_typed_var].
       iApply sem_typed_sub_u2aarr.
       iApply sem_typed_val. iApply resume_task_typed. }
     set resume_task := ("resume_task", resume_task_ty θ').
     rewrite -/next -/resume_task -/add.
-    iApply (sem_typed_let _ _ _ _ [main]); solve_sidecond.
+    smart_apply (sem_typed_let _ _ _ _ [main]).
     - assert (Hrw : [resume_task;add;next;main] = [resume_task;add;next] ++ [main]) by done.
       rewrite Hrw. clear Hrw.
       iApply sem_typed_sub_nil.
       iApply sem_typed_oval.
-      iApply (sem_typed_ufun_poly_rec 
-                (λ β, Promise ('! β) θ') 
-                (λ _, ⊥) 
-                (λ β, (() -{ coop θ' }-∘ '! β) -{ θ' }-∘ ())); solve_sidecond.
-     { iIntros. iApply copy_ty_uarr. }
-     simpl.
-     iIntros (β) "/=". 
-     set promise := ("promise", Promise ('! β) θ').
-     set fulfill := ("fulfill", ∀T: β', Promise ('! β') θ' → (() -{ coop θ' }-∘ '! β') -{ θ' }-∘ ()).
+      smart_apply (sem_typed_ufun_poly_rec 
+                  (λ β, Promise (! β) θ') 
+                  (λ _, ⊥) 
+                  (λ β, (𝟙 -{ coop θ' }-∘ ! β) -{ θ' }-∘ 𝟙)).
+     simpl. iIntros (β) "/=". 
+     set promise := ("promise", Promise (! β) θ').
+     set fulfill := ("fulfill", ∀ₜ β', Promise (! β') θ' → (𝟙 -{ coop θ' }-∘ ! β') -{ θ' }-∘ 𝟙).
      rewrite -(app_nil_r [promise;fulfill;resume_task;add;next]).
-     iApply sem_typed_afun; solve_sidecond. simpl.
-     set comp := ("comp", () -{ coop θ' }-∘ '! β)%T.
+     smart_apply sem_typed_afun. simpl.
+     set comp := ("comp", 𝟙 -{ coop θ' }-∘ ! β)%T.
      replace ([comp; promise; fulfill; resume_task; add;next]) with
              ([comp] ++ [promise; fulfill; resume_task; add;next]) by done.
-     iApply (sem_typed_handler2 (TT:=[tele _]) OS "async" "await" 
-                    (tele_app (λ α, () -{ coop θ' }-∘ '! α)) 
-                    (tele_app (λ α, Promise ('! α) θ')) 
-                    (tele_app (λ α, Promise ('! α) θ')) 
-                    (tele_app (λ α, '! α))  _ _ _ _ [comp] []); solve_sidecond.
-     + iIntros. iApply copy_ty_uarr.
-     + iIntros. iApply copy_ty_uarr.
+     smart_apply (sem_typed_handler2 (TT:=[tele _]) OS "async" "await" 
+                    (tele_app (λ α, 𝟙 -{ coop θ' }-∘ ! α)) 
+                    (tele_app (λ α, Promise (! α) θ')) 
+                    (tele_app (λ α, Promise (! α) θ')) 
+                    (tele_app (λ α, ! α))  _ _ _ _ [comp] []).
      + iApply row_le_refl.
-     + iApply (sem_typed_app_ms () _ ('! β)); try solve_copy; [iApply sem_typed_var'|].
+     + iApply (sem_typed_app_ms 𝟙 _ (! β)); [iApply sem_typed_var'|].
        rewrite -/(async_sig θ' (coop θ')) -/(await_sig θ') -/(coop_pre θ' (coop θ')).
        iApply sem_typed_sub_env_final.
        { iApply env_le_cons; first iApply env_le_refl. iApply ty_le_arr; try iApply ty_le_refl.
@@ -430,51 +414,51 @@ Section typing.
      + iIntros (β').
        iApply sem_typed_swap_third. iApply sem_typed_weaken.
        iApply sem_typed_swap_fourth. iApply sem_typed_weaken.
-       set x := ("x", () -{ coop θ' }-∘ '! β').
-       set k := ("k", Promise ('!β') θ' -{ θ' }-∘ ()).
+       set x := ("x", 𝟙 -{ coop θ' }-∘ ! β').
+       set k := ("k", Promise (!β') θ' -{ θ' }-∘ 𝟙).
        rewrite -/x -/k -/fulfill -/add -/next.
-       iApply (sem_typed_let (Promise ('! β') θ') _ _ _ [x;k;fulfill;add;next]); solve_sidecond. 
+       smart_apply (sem_typed_let (Promise (! β') θ') _ _ _ [x;k;fulfill;add;next]).
        { iApply sem_typed_alloc_cpy. iApply sem_typed_right_inj. iApply sem_typed_sub_nil. iApply sem_typed_nil. }
-       set new_prom := ("new_prom", Promise ('! β') θ'). 
+       set new_prom := ("new_prom", Promise (! β') θ'). 
        iApply (sem_typed_seq _ _ _ _ [new_prom; k; next]).
        * iApply sem_typed_sub_nil.
-         iApply (sem_typed_app_os (() -{ θ' }-∘ ())%T _ () _ [new_prom; k; add; next]).
+         iApply (sem_typed_app_os (𝟙 -{ θ' }-∘ 𝟙)%T _ 𝟙 _ [new_prom; k; add; next]).
          { iApply sem_typed_swap_third. iApply sem_typed_sub_u2aarr. iApply sem_typed_var'. }
          iApply sem_typed_swap_fourth. iApply sem_typed_swap_second.
-         iApply sem_typed_contraction; solve_sidecond.
+         iApply sem_typed_contraction.
          do 2 iApply sem_typed_swap_fourth.
          assert (Hrw : [fulfill; x; new_prom; new_prom; k; add; next] = 
                        [fulfill; x; new_prom] ++ [new_prom; k; add; next]) by done.
          rewrite Hrw. clear Hrw.
-         iApply sem_typed_afun; solve_sidecond. simpl.
+         smart_apply sem_typed_afun. simpl.
          iApply sem_typed_swap_second. iApply sem_typed_app_nil; last iApply sem_typed_var'.
          iApply sem_typed_swap_second. iApply sem_typed_app_os; last iApply sem_typed_var'.
-         set C := (λ β, Promise ('! β) θ' → (() -{ coop θ' }-∘ '! β) -{ θ' }-∘ ())%T.
+         set C := (λ β, Promise (! β) θ' → (𝟙 -{ coop θ' }-∘ ! β) -{ θ' }-∘ 𝟙)%T.
          iApply sem_typed_sub_u2aarr. rewrite -/(C β').
-         iApply sem_typed_TApp; first solve_copy. iApply sem_typed_var.
+         iApply sem_typed_TApp. iApply sem_typed_var.
       * simpl.
         iApply sem_typed_swap_third. iApply sem_typed_weaken.
-        iApply (sem_typed_app_ms (Promise ('! β') θ')); solve_sidecond; iApply sem_typed_var'.
+        iApply (sem_typed_app_ms (Promise (! β') θ')); iApply sem_typed_var'.
      + iIntros (β').
-       set x := ("x", Promise ('! β') θ').
-       set k := ("k", '! β' -{ θ' }-∘ ()).
+       set x := ("x", Promise (! β') θ').
+       set k := ("k", ! β' -{ θ' }-∘ 𝟙).
        do 4 (iApply sem_typed_swap_third; iApply sem_typed_weaken).
-       iApply (sem_typed_match ('! β') _ _  _ _ [x;k;next]); solve_sidecond.
+       smart_apply (sem_typed_match (! β') _ _  _ _ [x;k;next]).
        * iApply sem_typed_sub_nil.
          iApply sem_typed_replace_cpy_os; first iApply sem_typed_var.
-         iApply sem_typed_contraction; solve_sidecond.
+         iApply sem_typed_contraction.
          iApply sem_typed_right_inj. iApply sem_typed_nil.
-       * simpl. set v := ("v", '! β').
+       * simpl. set v := ("v", ! β').
          iApply sem_typed_swap_fourth. iApply sem_typed_weaken.
-         iApply sem_typed_contraction; solve_sidecond.
+         iApply sem_typed_contraction.
          iApply sem_typed_swap_third. iApply sem_typed_swap_second.
          iApply (sem_typed_seq _ _ _ _ [v; k]).
          { iApply sem_typed_sub_nil.
            iApply sem_typed_replace_cpy_os; [iApply sem_typed_var|].
            iApply sem_typed_left_inj. iApply sem_typed_var. }
-         iApply (sem_typed_app_ms ('! β')); solve_sidecond; iApply sem_typed_var'.
-       * simpl. set ks := ("ks", List ('! β' -{ θ' }-∘ ())).
-         iApply (sem_typed_seq (Status ('! β') θ')).
+         iApply (sem_typed_app_ms (! β')); iApply sem_typed_var'.
+       * simpl. set ks := ("ks", List (! β' -{ θ' }-∘ 𝟙)).
+         iApply (sem_typed_seq (Status (! β') θ')).
          ** iApply sem_typed_swap_third. 
             iApply sem_typed_sub_nil.
             iApply sem_typed_replace_cpy_os; first iApply sem_typed_var'.
@@ -484,71 +468,70 @@ Section typing.
             assert (Hrw : [k; x; next] = [k] ++ [x;next]) by done.
             rewrite Hrw. clear Hrw.
             iApply sem_typed_var.
-          ** iApply (sem_typed_app_ms ()); solve_sidecond; [|iApply sem_typed_unit'].
+          ** iApply (sem_typed_app_ms 𝟙); [|iApply sem_typed_unit'].
              iApply sem_typed_sub_u2aarr; iApply sem_typed_var'.
     + simpl. 
       iApply sem_typed_swap_third. iApply sem_typed_weaken.
       iApply sem_typed_swap_fourth; iApply sem_typed_weaken.
       iApply sem_typed_swap_second.
-      set x := ("x", '!β). rewrite -/resume_task -/promise.
-      iApply (sem_typed_let _ _ _ _ [promise; x; resume_task; next]); solve_sidecond.
+      set x := ("x", !β). rewrite -/resume_task -/promise.
+      smart_apply (sem_typed_let _ _ _ _ [promise; x; resume_task; next]).
       * iApply sem_typed_sub_nil.
         iApply sem_typed_replace_cpy_os; [|iApply sem_typed_right_inj; iApply sem_typed_nil].
-        iApply sem_typed_contraction; solve_sidecond.
+        iApply sem_typed_contraction.
         iApply sem_typed_var.
-      * set v := ("v", '! β + (List ('! β -{ θ' }-∘ ()))).
-        iApply (sem_typed_match  _ _ _ _ _ [promise; x; resume_task; next]); solve_sidecond;
-          [iApply sem_typed_var'| |].
+      * set v := ("v", ! β + (List (! β -{ θ' }-∘ 𝟙))).
+        smart_apply (sem_typed_match  _ _ _ _ _ [promise; x; resume_task; next]); [iApply sem_typed_var'| |].
         { simpl. do 4 (iApply sem_typed_weaken). iApply sem_typed_sub_nil. iApply impossible_typed. }
         simpl. iApply sem_typed_swap_second. 
-        iApply sem_typed_swap_third. iApply sem_typed_contraction; solve_sidecond.
+        iApply sem_typed_swap_third. iApply sem_typed_contraction.
         iApply sem_typed_swap_third. iApply sem_typed_swap_second.
-        set ks := ("ks", List ('! β -{ θ' }-∘ ())).
+        set ks := ("ks", List (! β -{ θ' }-∘ 𝟙)).
         iApply (sem_typed_seq _ _ _ _ [x; ks; resume_task; next]).
         ** iApply sem_typed_sub_nil.
            iApply sem_typed_replace_cpy_os; [iApply sem_typed_var|].
            iApply sem_typed_left_inj. iApply sem_typed_var.
-        ** iApply (sem_typed_seq ()).
-           2: { iApply (sem_typed_app_ms ()); solve_sidecond; [|iApply sem_typed_unit'].
+        ** iApply (sem_typed_seq 𝟙).
+           2: { iApply (sem_typed_app_ms 𝟙); [|iApply sem_typed_unit'].
                 iApply sem_typed_sub_u2aarr; iApply sem_typed_var'. }
            iApply sem_typed_swap_second.
            iApply sem_typed_sub_nil.
            iApply sem_typed_app_os; [|iApply sem_typed_var].
-           iApply (sem_typed_app_os (('! β -{ θ' }-∘ ()) → ())%T).
+           iApply (sem_typed_app_os ((! β -{ θ' }-∘ 𝟙) → 𝟙)%T).
            2: { iApply sem_typed_app_os; [|iApply sem_typed_var]. 
                 iApply sem_typed_sub_u2aarr.
-                set C := λ β, ('! β → ('! β -{ θ' }-∘ ()) → ())%T. rewrite -/(C β). simpl.
-                iApply sem_typed_TApp; first solve_sidecond. iApply sem_typed_var. }
+                set C := λ β, (! β → (! β -{ θ' }-∘ 𝟙) → 𝟙)%T. rewrite -/(C β). simpl.
+                iApply sem_typed_TApp. iApply sem_typed_var. }
            iApply sem_typed_sub_u2aarr.
            iApply sem_typed_sub_ty; first iApply ty_le_uarr; 
             [iApply row_le_refl|iApply ty_le_uarr|iApply ty_le_refl|];
             [iApply (row_le_mfbang_intro OS)|iApply ty_le_refl|iApply ty_le_refl|].
            iApply sem_typed_sub_ty; first iApply ty_le_uarr; 
             [iApply row_le_refl|iApply ty_le_refl|iApply ty_le_arr|];
-            [iApply (row_le_mfbang_elim OS)|iApply ty_le_refl|iApply ty_le_refl|].
-            set C := (λ (θ : sem_row Σ), (('! β -{ θ' }-∘ ()) -{ ¡ θ }-> ()) → List ('! β -{θ'}-∘ ()) -{ ¡ θ }-∘ ())%T.
+            [iApply (@row_le_mfbang_elim _ _)|iApply ty_le_refl|iApply ty_le_refl|].
+            set C := (λ (θ : sem_row Σ), ((! β -{ θ' }-∘ 𝟙) -{ ¡ θ }-> 𝟙) → List (! β -{θ'}-∘ 𝟙) -{ ¡ θ }-∘ 𝟙)%T.
            rewrite -/(C ⊥).
-           iApply sem_typed_RApp; first solve_copy. 
+           iApply sem_typed_RApp.
            iApply sem_typed_val. iApply iter_typed.
-  - set fulfill := ("fulfill", ∀T: α, Promise ('! α) θ' → (() -{ coop θ' }-∘ '! α) -{ θ' }-∘ ()).
-    iApply (sem_typed_let _ _ _ _ [fulfill; main]); solve_sidecond.
-    { iApply (sem_typed_alloc_cpy (Status ('! α) θ')). 
+  - set fulfill := ("fulfill", ∀ₜ α, Promise (! α) θ' → (𝟙 -{ coop θ' }-∘ ! α) -{ θ' }-∘ 𝟙).
+    smart_apply (sem_typed_let _ _ _ _ [fulfill; main]).
+    { iApply (sem_typed_alloc_cpy (Status (! α) θ')). 
       iApply sem_typed_right_inj. iApply sem_typed_sub_nil. iApply sem_typed_nil. }
-    set pmain := ("pmain", Refᶜ Status ('! α) θ').
-    iApply sem_typed_contraction; solve_sidecond.
+    set pmain := ("pmain", Refᶜ Status (! α) θ').
+    iApply sem_typed_contraction.
     iApply sem_typed_swap_third. iApply sem_typed_swap_second. iApply sem_typed_swap_fourth.
-    iApply (sem_typed_seq ()).
-    + iApply sem_typed_swap_second. iApply sem_typed_frame_ms; solve_copy.
+    iApply (sem_typed_seq 𝟙).
+    + iApply sem_typed_swap_second. iApply sem_typed_frame_ms.
       iApply sem_typed_app_nil; last iApply sem_typed_var'.
       iApply sem_typed_swap_second.
       iApply sem_typed_app_os; last iApply sem_typed_var'.
       iApply sem_typed_sub_u2aarr. 
-      set C := (λ α, Promise ('! α) θ' → (() -{ coop θ' }-∘ '! α) -{ θ' }-∘ ())%T.
-      rewrite -/(Promise ('! α) θ') -/(C α).
+      set C := (λ α, Promise (! α) θ' → (𝟙 -{ coop θ' }-∘ ! α) -{ θ' }-∘ 𝟙)%T.
+      rewrite -/(Promise (! α) θ') -/(C α).
       iApply sem_typed_TApp. rewrite /C /Promise.
       iApply sem_typed_var'.
     + iApply sem_typed_sub_nil.
-      iApply (sem_typed_match _ _ _ _ _ []); solve_sidecond; simpl; [|iApply sem_typed_var|].
+      smart_apply (sem_typed_match _ _ _ _ _ []); simpl; [|iApply sem_typed_var|].
       { iApply sem_typed_replace_cpy_os; [iApply sem_typed_var|].
         iApply sem_typed_right_inj. iApply sem_typed_nil. }
       iApply impossible_typed. 
@@ -557,59 +540,59 @@ Section typing.
   Definition coopstate : sem_row Σ := coop st.
 
   Lemma prog_typed :
-    ⊢ ⊨ prog : st : ().
+    ⊢ ⊨ prog : st : 𝟙.
   Proof.
     rewrite /prog. iIntros.
-    iApply (sem_typed_app_nil (() -{ coopstate }-∘ ())).
+    iApply (sem_typed_app_nil (𝟙 -{ coopstate }-∘ 𝟙)).
     - iApply sem_typed_sub_ty; first iApply ty_le_u2aarr.
       iApply sem_typed_sub_ty.
       { iApply ty_le_uarr; [iApply row_le_refl| |iApply (ty_le_mbang_elim MS)].
-        iApply ty_le_arr; [iApply row_le_refl|iApply ty_le_refl|iApply (ty_le_mbang_intro MS); solve_copy]. }
-      set R := (λ α θ', (() -{ coop θ' }-∘ '! α) -{ θ' }-> '! α)%T.
-      rewrite /coopstate -/(R () st).
-      iApply (sem_typed_RApp (R ())).
-      iApply (sem_typed_TApp (λ α, ∀R: θ, R α θ)).
+        iApply ty_le_arr; [iApply row_le_refl|iApply ty_le_refl|iApply (ty_le_mbang_intro_unit)]. }
+      set R := (λ α θ', (𝟙 -{ coop θ' }-∘ ! α) -{ θ' }-> ! α)%T.
+      rewrite /coopstate -/(R 𝟙 st).
+      iApply (sem_typed_RApp (R 𝟙)).
+      iApply (sem_typed_TApp (λ α, ∀ᵣ θ, R α θ)).
       iApply sem_typed_val. iApply runner_typed.
     - rewrite - {1} (app_nil_r []).
       iApply sem_typed_sub_nil.
-      iApply sem_typed_afun; solve_sidecond. simpl.
-      iApply (sem_typed_seq ()).
+      smart_apply sem_typed_afun. simpl.
+      iApply (sem_typed_seq 𝟙).
       + rewrite /coopstate /coop.
         iApply sem_typed_sub_row; first iApply row_le_rec_fold.
         rewrite -/(coop st) {1} /coop_pre {7} /st.
         iApply sem_typed_sub_row; first iApply row_le_swap_third; try done.
         iApply sem_typed_sub_row; first iApply row_le_swap_second; try done.
-        iApply (sem_typed_perform_ms (TT:=[tele _]) [tele_arg ()] with "[] []"); first solve_copy.
+        iApply (sem_typed_perform_ms (TT:=[tele _]) [tele_arg 𝟙] with "[]").
         iApply sem_typed_int'.
-      + set p1type := (Promise ('! ())%T st).
-        iApply (sem_typed_let p1type _ _ _  []); solve_sidecond.
-        * set A := (λ α θ', (() -{ coop θ' }-∘ '! α) -{ coop θ' }-> Promise ('! α) θ')%T.
-          iApply (sem_typed_app_nil (() -{ coopstate }-∘ '! ())).
+      + set p1type := (Promise (! 𝟙)%T st).
+        smart_apply (sem_typed_let p1type _ _ _  []).
+        * set A := (λ α θ', (𝟙 -{ coop θ' }-∘ ! α) -{ coop θ' }-> Promise (! α) θ')%T.
+          iApply (sem_typed_app_nil (𝟙 -{ coopstate }-∘ ! 𝟙)).
           { iApply sem_typed_sub_ty; first iApply ty_le_u2aarr.
-            rewrite /coopstate /p1type -/(A () st).
+            rewrite /coopstate /p1type -/(A 𝟙 st).
             iApply (sem_typed_TApp (λ α, A α st)).
-            iApply (sem_typed_RApp (λ θ', ∀T: α, A α θ')).
+            iApply (sem_typed_RApp (λ θ', ∀ₜ α, A α θ')).
             iApply sem_typed_val. iApply async_typed. }
           iApply sem_typed_sub_nil. rewrite - {1} (app_nil_r []).
-          iApply sem_typed_afun; solve_sidecond. simpl.
+          smart_apply sem_typed_afun. simpl.
           iApply sem_typed_sub_row; first iApply row_le_rec_fold.
           rewrite -/(coop st) {1} /coop_pre {7} /st.
           iApply sem_typed_sub_row; first iApply row_le_swap_third; try done.
           iApply sem_typed_sub_row; first iApply row_le_swap_second; try done.
-          iApply sem_typed_sub_ty; first iApply (ty_le_mbang_intro MS); first solve_copy.
-          iApply (sem_typed_perform_ms (TT:=[tele _]) [tele_arg ()] with "[] []"); solve_sidecond.
+          iApply sem_typed_sub_ty; first iApply (ty_le_mbang_intro_unit).
+          iApply (sem_typed_perform_ms (TT:=[tele _]) [tele_arg 𝟙] with "[]").
           iApply sem_typed_sub_row; first iApply row_le_swap_fourth; try done.
           do 2 (iApply sem_typed_sub_row; first iApply row_le_swap_third; try done).
           iApply (sem_typed_bin_op ℤ ℤ ℤ); [constructor| |iApply sem_typed_int'].
-          iApply (sem_typed_perform_ms (TT:=[tele _]) [tele_arg ()] with "[] []"); solve_sidecond.
+          iApply (sem_typed_perform_ms (TT:=[tele _]) [tele_arg 𝟙] with "[]").
           iApply sem_typed_unit'.
-        * set A := (λ α θ', Promise ('! α) θ' -{ coop θ' }-> '! α)%T.
+        * set A := (λ α θ', Promise (! α) θ' -{ coop θ' }-> ! α)%T.
           iApply (sem_typed_app_nil p1type).
           { iApply sem_typed_sub_ty; first iApply ty_le_u2aarr.
             iApply sem_typed_sub_ty; first iApply ty_le_uarr; [iApply row_le_refl|iApply ty_le_refl|iApply (ty_le_mbang_elim MS)| ].
-            rewrite /coopstate /p1type -/(A () st).
+            rewrite /coopstate /p1type -/(A 𝟙 st).
             iApply (sem_typed_TApp (λ α, A α st)).
-            iApply (sem_typed_RApp (λ θ', ∀T: α, A α θ')).
+            iApply (sem_typed_RApp (λ θ', ∀ₜ α, A α θ')).
             iApply sem_typed_val. iApply await_typed. }
           iApply sem_typed_var'.
   Qed.
